Update sorting.dfy

LAB2/Sorting/sorting.dfy
@@ -1,44 +1,53 @@
 class sorting{
 
-    predicate sorted(s: seq<int>)
-    reads this;
-    {
-      forall i,j :: 0 <= i < j < |s| ==> s[i] <= s[j]
-    }
-    
-    predicate sorted2(s: seq<int>)
-    reads this;
-    {
-       0 < |s| ==> (forall i :: 0 < i < |s| ==> s[0] <= s[i]) &&
- sorted2(s[1..])
-    }
-    
-    //wtf does "if a sequence is sorted, then it is sorted" two times mean?????????`???????
-    ghost method IsSorted (s: seq<int>) 
-    requires |s| < 2
-    ensures sorted(s)
-    {
-      //...
-    }
-    
-     ghost method IsSorted2 (s: seq<int>) 
-    requires |s| < 2
-    ensures sorted2(s)
-    {
-      //...
-    }
-    
-    predicate p2(a : seq<int>, b : seq<int>)
-    reads this;
-    {
-      |a+b| == |a| + |b| 
-    }
-    
-  method badSpec(s: seq<int>)
-    requires |s| < 2;
-    //ensures  sorted(a[0..|a|);
-    ensures forall i,j :: 0 <= i < j < |s| ==> s[i] <= s[j]
-    {
-      
-    }
+predicate sorted(s: seq<int>)
+reads this;
+{
+forall i,j :: 0 <= i < j < |s| ==> s[i] <= s[j]
+}
+
+predicate sorted2(s: seq<int>)
+reads this;
+{
+0 < |s| ==> (forall i :: 0 < i < |s| ==> s[0] <= s[i]) &&
+sorted2(s[1..])
+}
+
+
+ghost method IsSorted (s: seq<int>)
+requires sorted2(s)
+ensures sorted(s)
+{
+//...
+}
+
+ghost method IsSorted2 (s: seq<int>)
+requires sorted(s);
+ensures sorted2(s)
+{
+//...
+}
+
+predicate p2(a : seq<int>, b : seq<int>)
+reads this;
+requires |a| == |b|;
+{
+forall i :: 0 <= i <|a| ==> a[i] == b[i]
+}
+
+method sortArray(a : array<int>)
+requires a != null;
+ensures sorted(a[..]);
+ensures p2(old(a[..]), a[..])
+{
+
+}
+
+
+method badSpec(a: array<int>)
+requires a != null;
+ensures forall sorted(a[..]);
+{
+
+}
 }
